\def\inputNum{-20220520}
\toks0{(11/(45-1) \times 4)}
\toks1{(-11+4-5+14)}
\toks2{(-11-4+5+14)}
\toks3{(11-4-5+14)}
\toks4{((114-51) \times 4+(-11-4+5+14))}
\toks5{(114 \times 514+(11 \times 45 \times 14+(-11/4+51/4)))}
\count0=\inputNum\relax
\def\loop#1#2#3{
    #3
    \ifnum #1<#2
        \advance#1 by 1
        \loop{#1}{#2}{#3}
    \fi
}
\def\homoBinary#1{
    \ifnum #1=0
        \the\toks0
    \else
        \count4=#1
        \count5=1
        \count6=0
        \loop{\count5}{6}{
            \ifodd\count4
                \ifnum\count6=1
                    \times
                \fi
                \count6=1
                \the\toks\count5
            \fi
            \divide\count4 by 2
        }
    \fi
}
\def\homo#1{
    \ifnum #1=0
        (1-1) \times 4514
    \else
        \ifnum #1>0
            \count1=\the#1
            \count2=0
            \count3=0
            \loop{\count2}{32}{
                \ifodd\count1
                    \ifnum\count3=1
                        +
                    \fi
                    \count3=1
                    \homoBinary{\count2}
                \fi
                \divide\count1 by 2
            }
        \else
            \count1=0
            \advance\count1 by -\count0
            \count0=\count1
            (11-4-5+1-4) \times (\homo{#1})
        \fi
    \fi
}
Ok, You input $\the\count0$.

Obviously, $\the\count0 = \homo{\count0}$

\bye
